Started work on InsertionSort

DeductiveVericoding/ListLanguage/Parametrized/InsertionSort.lean
@@ -1,7 +1,9 @@
 import Mathlib.Data.List.Perm.Basic
-import DeductiveVericoding.ListLanguage.Basic
+import DeductiveVericoding.ListLanguage.Parametrized.Tactics
 
 open ListLanguage
+
+namespace Parametrized
 
 def insertVal (a : Nat) : List Nat → List Nat
   | [] => [a]
@@ -13,12 +15,19 @@ def Ordered : List Nat → Prop
   | x :: y :: xs => x ≤ y ∧ Ordered (y :: xs)
 
 /-- The sorting invariant: output is sorted and a permutation of input -/
-def Sorted (inp out : List Nat) : Prop :=
-  Ordered out ∧ List.Perm inp out
+def Sorted (inp out : List Nat) : Prop := Ordered out ∧ (List.Perm inp out)
+
+/- ## Properties of the base case -/
+
+lemma NilSorted_iff (out : List Nat) : Sorted [] out ↔ out = [] := by
+  simp only [Sorted, List.nil_perm, and_iff_right_iff_imp]
+  intro h
+  rw [h]
+  trivial
 
 /-! ## Properties of insertVal -/
 
-theorem insertVal_sorted (a : Nat) (l : List Nat) (hs : Ordered l) :
+theorem insertVal_ordered (a : Nat) (l : List Nat) (hs : Ordered l) :
     Ordered (insertVal a l) := by
   induction l with
   | nil => trivial
@@ -61,3 +70,62 @@ theorem insertVal_le_cons (a h : Nat) (t : List Nat) (hs : Ordered (h :: t)) (hl
     have hh' : h ≤ h' := hs.1
     have hah' : a ≤ h' := Nat.le_trans hle hh'
     simp [hah']
+
+/- # Sorting as a function -/
+
+lemma Perm_trans {l1 l2 l3 : List Nat} : l1.Perm l2 → l2.Perm l3 → l1.Perm l3 := by
+  sorry
+
+lemma exists_sorted (inp : List Nat) : ∃! out, Sorted inp out := by
+  induction inp with
+  | nil => simp only [NilSorted_iff, existsUnique_eq]
+  | cons a l ih =>
+    obtain ⟨l', h1, h2⟩ := ih
+    refine ⟨(insertVal a l'), ⟨insertVal_ordered a l' h1.1, ?_⟩, ?_⟩
+    · apply Perm_trans (List.Perm.cons a h1.2) (insertVal_perm a l')
+    sorry
+
+noncomputable def sorted (l : List Nat) : List Nat := Classical.choose <| exists_sorted l
+
+lemma Sorted_iff_eq_sorted (inp out : List Nat) : Sorted inp out ↔ out = sorted inp := by
+  obtain ⟨out', h1, h2⟩ := exists_sorted inp
+  refine ⟨fun h ↦ (Classical.choose_spec (exists_sorted inp)).2 _ h, fun h ↦ ?_⟩
+  rw [h]
+  apply (Classical.choose_spec (exists_sorted inp)).1
+
+lemma sorted_cons (a : Nat) (l : List Nat) : sorted (a :: l) = insertVal a (sorted l) := by
+  sorry
+
+/- # InsertionSort Vericoding -/
+
+abbrev InsertionSortProblem := ImplP [] (.arrow .list .list) (fun _ f ↦ ∀ l, Sorted l (f l))
+
+abbrev InsertProblem := ImplP [] (.arrow .nat (.arrow .list .list)) (fun _ f ↦ ∀ a, ∀ l, Ordered l → Sorted (a :: l) (f a l))
+
+def InsertionSolution : InsertProblem := by
+  introP
+  listRecP
+  · simp [Sorted, Ordered]
+    apply RelaxCondPTactic (t:=.list) _ (fun env out => out = [(env.getT 0 .nat)])
+    · apply ConsPTactic
+      · apply ParPTactic
+      apply NilPTactic
+    simp only [forall_eq, Ordered, and_self, implies_true]
+  sorry
+
+
+
+
+def InsertionSortSolution : InsertionSortProblem := by
+  listRecP
+  · simp [NilSorted_iff]
+    apply NilPTactic
+  simp [Sorted_iff_eq_sorted, sorted_cons]
+  pushpreP
+  apply AppPTactic _ .list .list (fun env => env.getT 2 .list) (fun env l out => out = insertVal (env.getT 0 Tpe.nat) l)
+  · apply ParPTactic
+  listRecP
+  · apply ConsPTactic
+    · apply ParPTactic
+    apply NilPTactic
+  sorry
